

Maths behind Ridge Regression

$$L = \sum_{i=1}^n (Y_i - \hat{Y}_i)^2 + \lambda m^2$$

where $m = \text{slope} \dots$

$$b = \bar{Y} - m\bar{X}$$

$$L = \sum_{i=1}^n (Y_i - mX_i - b)^2 + \lambda m^2$$

$$\frac{\partial L}{\partial m} = \frac{\partial}{\partial m} \sum_{i=1}^n (Y_i - mX_i - \bar{Y} + m\bar{X})^2 + \lambda m^2$$

$$\frac{\partial L}{\partial m} \Rightarrow 2 \sum_{i=1}^n (Y_i - mX_i - \bar{Y} + m\bar{X}) (-X_i + \bar{X}) + 2\lambda m = 0$$

$$\Rightarrow \sum_{i=1}^n (Y_i - \bar{Y} - mX_i + m\bar{X}) \cdot (X_i - \bar{X}) + \lambda m = 0$$

$$\Rightarrow \lambda m - \sum_{i=1}^n [(Y_i - \bar{Y}) - m(X_i - \bar{X})] \cdot (X_i - \bar{X}) = 0$$

$$\Rightarrow \lambda m - \sum_{i=1}^n (Y_i - \bar{Y})(X_i - \bar{X}) + m \sum_{i=1}^n (X_i - \bar{X})^2 = 0$$

$$\Rightarrow \lambda m - \sum_{i=1}^n (Y_i - \bar{Y})(X_i - \bar{X}) + m \sum_{i=1}^n (X_i - \bar{X})^2 = 0$$

$$\Rightarrow \lambda m + m \sum_{i=1}^n (X_i - \bar{X})^2 = \sum_{i=1}^n (Y_i - \bar{Y})(X_i - \bar{X})$$

$$\downarrow m = \frac{\sum_{i=1}^n (Y_i - \bar{Y})(X_i - \bar{X})}{\sum_{i=1}^n (X_i - \bar{X})^2 + \lambda}$$

hyper parameter also known as "alpha"

As the Value of λ Alpha Increases,the Value of m decreases....